SyBloc/SBSemantics.v
@@ -29,15 +29,13 @@ Module Type SBSEMANTICS
   Definition history := PM.t (stream value).
 
   Record mvalue :=
-    Mvalue { content_i: value;
-             reset_i: bool;
-             init_i: const
+    Mvalue { content_i: val;
+             reset_i: bool
            }.
 
   Record mvalues :=
-    Mvalues { content: stream value;
-              reset: stream bool;
-              init: const
+    Mvalues { content: stream val;
+              reset: stream bool
             }.
 
   Definition memory := RMemory.memory mvalue.
@@ -51,33 +49,18 @@ Module Type SBSEMANTICS
   (*     then Some (snd m) else find_init x mems *)
   (*   end. *)
 
-  Definition get_reg (x: ident) (m: memory) :=
-      match mfind_mem x m with
-      | Some mv =>
-        Some (if mv.(reset_i) then present (sem_const mv.(init_i))
-              else mv.(content_i))
-      | None => None
-      end.
-
   (** ** Instantaneous semantics *)
 
   Section InstantSemantics.
 
     Variable base: bool.
     Variable R: env.
-    Variable m: memory.
 
     Inductive sem_var_instant: ident -> value -> Prop :=
       Sv:
         forall x v,
           PM.find x R = Some v ->
           sem_var_instant x v.
-
-    Inductive sem_mem_var_instant: ident -> value -> Prop :=
-      Smv:
-        forall x v,
-          get_reg x m = Some v ->
-          sem_mem_var_instant x v.
 
     Inductive sem_clock_instant: clock -> bool -> Prop :=
     | Sbase:
@@ -109,10 +92,6 @@ Module Type SBSEMANTICS
         forall x v ty,
           sem_var_instant x v ->
           sem_lexp_instant (Evar x ty) v
-    | Sreg:
-        forall x v ty,
-          sem_mem_var_instant x v ->
-          sem_lexp_instant (Ereg x ty) v
     | Swhen_eq:
         forall s x sc xc b,
           sem_var_instant x (present xc) ->
@@ -197,19 +176,18 @@ Module Type SBSEMANTICS
 
     Variable base : bool.
     Variable R: env.
-    Variable m: memory.
 
     Inductive sem_annotated_instant {A}
-              (sem_instant: bool -> env -> memory -> A -> value -> Prop)
+              (sem_instant: bool -> env -> A -> value -> Prop)
       : clock -> A -> value -> Prop :=
     | Stick:
         forall ck a c,
-          sem_instant base R m a (present c) ->
+          sem_instant base R a (present c) ->
           sem_clock_instant base R ck true ->
           sem_annotated_instant sem_instant ck a (present c)
     | Sabs:
         forall ck a,
-          sem_instant base R m a absent ->
+          sem_instant base R a absent ->
           sem_clock_instant base R ck false ->
           sem_annotated_instant sem_instant ck a absent.
 
@@ -220,13 +198,13 @@ Module Type SBSEMANTICS
     | SLticks:
         forall ck ces cs vs,
           vs = map present cs ->
-          sem_lexps_instant base R m ces vs ->
+          sem_lexps_instant base R ces vs ->
           sem_clock_instant base R ck true ->
           sem_laexps_instant ck ces vs
     | SLabss:
         forall ck ces vs,
           vs = all_absent ces ->
-          sem_lexps_instant base R m ces vs ->
+          sem_lexps_instant base R ces vs ->
           sem_clock_instant base R ck false ->
           sem_laexps_instant ck ces vs
     | SNil:
@@ -241,22 +219,14 @@ Module Type SBSEMANTICS
 
     Variable bk : stream bool.
     Variable H : history.
-    Variable M: memories.
 
     Definition restr_hist (n: nat): env :=
       PM.map (fun xs => xs n) H.
     Hint Unfold restr_hist.
 
-    Definition restr_mvalues (n: nat) (mvs: mvalues): mvalue :=
-      {| content_i := mvs.(content) n; reset_i := mvs.(reset) n; init_i := mvs.(init) |}.
-
-    Definition restr_mem (n: nat): memory :=
-      mmap (restr_mvalues n) M.
-    Hint Unfold restr_mem.
-
-    Definition lift {A B} (sem: bool -> env -> memory -> A -> B -> Prop)
+    Definition lift {A B} (sem: bool -> env -> A -> B -> Prop)
                x (ys: stream B): Prop :=
-      forall n, sem (bk n) (restr_hist n) (restr_mem n) x (ys n).
+      forall n, sem (bk n) (restr_hist n) x (ys n).
     Hint Unfold lift.
 
     Definition lift' {A B} (sem: bool -> env -> A -> B -> Prop) x (ys: stream B): Prop :=
@@ -277,10 +247,10 @@ Module Type SBSEMANTICS
       lift'' (fun R => Forall2 (sem_var_instant R)) x xs.
 
     Definition sem_laexp ck (e: lexp) (xs: stream value): Prop :=
-      lift (fun base R m => sem_laexp_instant base R m ck) e xs.
+      lift (fun base R => sem_laexp_instant base R ck) e xs.
 
     Definition sem_laexps (ck: clock) (e: list lexp) (xs: stream (list value)): Prop :=
-      lift (fun base R m => sem_laexps_instant base R m ck) e xs.
+      lift (fun base R => sem_laexps_instant base R ck) e xs.
 
     Definition sem_lexp (e: lexp) (xs: stream value): Prop :=
       lift sem_lexp_instant e xs.
@@ -289,7 +259,7 @@ Module Type SBSEMANTICS
       lift sem_lexps_instant e xs.
 
     Definition sem_caexp ck (c: cexp) (xs: stream value): Prop :=
-      lift (fun base R m => sem_caexp_instant base R m ck) c xs.
+      lift (fun base R => sem_caexp_instant base R ck) c xs.
 
     Definition sem_cexp (c: cexp) (xs: stream value): Prop :=
       lift sem_cexp_instant c xs.
@@ -308,41 +278,41 @@ Module Type SBSEMANTICS
     forall n,
       present_list (xss n) <-> bs n = true.
 
-  (* Definition clock_of' (xss: stream (list value)) : stream bool := *)
-  (*   fun n => forallb (fun v => negb (v ==b absent)) (xss n). *)
+  Definition clock_of' (xss: stream (list value)) : stream bool :=
+    fun n => forallb (fun v => negb (v ==b absent)) (xss n).
 
-  (* Lemma clock_of_equiv: *)
-  (*   forall xss, clock_of xss (clock_of' xss). *)
-  (* Proof. *)
-  (*   split; intros H. *)
-  (*   - unfold clock_of'. *)
-  (*     rewrite forallb_forall. *)
-  (*     intros; rewrite Bool.negb_true_iff. *)
-  (*     rewrite not_equiv_decb_equiv. *)
-  (*     eapply In_Forall in H; eauto. *)
-  (*   - unfold clock_of' in H. *)
-  (*     rewrite forallb_forall in H. *)
-  (*     apply all_In_Forall; intros ** Hin E. *)
-  (*     specialize (H _ Hin). *)
-  (*     rewrite Bool.negb_true_iff, not_equiv_decb_equiv in H. *)
-  (*     apply H; eauto. *)
-  (* Qed. *)
+  Lemma clock_of_equiv:
+    forall xss, clock_of xss (clock_of' xss).
+  Proof.
+    split; intros H.
+    - unfold clock_of'.
+      rewrite forallb_forall.
+      intros; rewrite Bool.negb_true_iff.
+      rewrite not_equiv_decb_equiv.
+      eapply In_Forall in H; eauto.
+    - unfold clock_of' in H.
+      rewrite forallb_forall in H.
+      apply all_In_Forall; intros ** Hin E.
+      specialize (H _ Hin).
+      rewrite Bool.negb_true_iff, not_equiv_decb_equiv in H.
+      apply H; eauto.
+  Qed.
 
-  Inductive next_reg: ident -> stream value -> memories -> Prop :=
-    post_mem_intro:
-      forall x xs M mvs,
-        mfind_mem x M = Some mvs ->
-        mvs.(content) ≈ fby (sem_const mvs.(init)) xs ->
-        next_reg x xs M .
+  (* Inductive next_reg: ident -> stream value -> memories -> Prop := *)
+  (*   post_mem_intro: *)
+  (*     forall x xs M mvs, *)
+  (*       mfind_mem x M = Some mvs -> *)
+  (*       mvs.(content) ≈ fby (sem_const mvs.(init)) xs -> *)
+  (*       next_reg x xs M . *)
 
   Inductive reset_regs: stream bool -> memories -> Prop :=
     reset_regs_intro:
       forall M rs,
         (forall x mvs,
-            mfind_mem x M = Some mvs ->
+            find_val x M = Some mvs ->
             forall n, rs n = true -> mvs.(reset) n = true) ->
         (forall x M',
-            mfind_inst x M = Some M' ->
+            find_inst x M = Some M' ->
             reset_regs rs M') ->
         reset_regs rs M.
 
@@ -353,6 +323,21 @@ Module Type SBSEMANTICS
       | _ => false
       end.
 
+  Inductive mfby: ident -> val -> stream value -> memories -> stream value -> Prop :=
+    mfby_intro:
+      forall x mvs v0 ls M xs,
+        find_val x M = Some mvs ->
+        mvs.(content) 0 = v0 ->
+        (forall n, match ls n with
+              | absent =>
+                mvs.(content) (S n) = (if mvs.(reset) (S n) then v0 else mvs.(content) n)
+                /\ xs n = absent
+              | present v =>
+                mvs.(content) (S n) = (if mvs.(reset) (S n) then v0 else v)
+                /\ xs n = present (mvs.(content) n)
+              end) ->
+        mfby x v0 ls M xs.
+
   Section BlockSemantics.
 
     Variable P: program.
@@ -361,13 +346,14 @@ Module Type SBSEMANTICS
     | SEqDef:
         forall bk H M x xs ck ce,
           sem_var H x xs ->
-          sem_caexp bk H M ck ce xs ->
+          sem_caexp bk H ck ce xs ->
           sem_equation bk H M (EqDef x ck ce)
-    | SEqReg:
-        forall bk H M x ck ce xs,
-          sem_caexp bk H M ck ce xs ->
-          next_reg x xs M ->
-          sem_equation bk H M (EqReg x ck ce)
+    | SEqFby:
+        forall bk H M x ck c0 e xs ls,
+          sem_var H x xs ->
+          sem_laexp bk H ck e ls ->
+          mfby x (sem_const c0) ls M xs ->
+          sem_equation bk H M (EqFby x ck c0 e)
     | SEqReset:
         forall bk H M ck b i r rs M',
           sem_var H r rs ->
@@ -376,7 +362,7 @@ Module Type SBSEMANTICS
           sem_equation bk H M (EqReset ck b i r)
     | SEqCall:
         forall bk H M ys M' ck b i es ess oss,
-          sem_laexps bk H M ck es ess ->
+          sem_laexps bk H ck es ess ->
           sub_inst i M M' ->
           sem_block b M' ess oss ->
           sem_vars H ys oss ->
@@ -396,5 +382,73 @@ Module Type SBSEMANTICS
                sem_block b M xss yss.
 
   End BlockSemantics.
+
+  Section sem_block_mult.
+    Variable P: program.
+
+    Variable P_equation: stream bool -> history -> memories -> equation -> Prop.
+    Variable P_block: ident -> memories -> stream (list value) -> stream (list value) -> Prop.
+
+    Hypothesis EqDefCase:
+      forall bk H M x xs ck ce,
+        sem_var H x xs ->
+        sem_caexp bk H ck ce xs ->
+        P_equation bk H M (EqDef x ck ce).
+
+    Hypothesis EqFbyCase:
+      forall bk H M x ck c0 e xs ls,
+        sem_var H x xs ->
+        sem_laexp bk H ck e ls ->
+        mfby x (sem_const c0) ls M xs ->
+        P_equation bk H M (EqFby x ck c0 e).
+
+    Hypothesis EqResetCase:
+      forall bk H M ck b i r rs M',
+        sem_var H r rs ->
+        sub_inst i M M' ->
+        reset_regs (reset_of rs) M' ->
+        P_equation bk H M (EqReset ck b i r).
+
+    Hypothesis EqCallCase:
+      forall bk H M ys M' ck b i es ess oss,
+        sem_laexps bk H ck es ess ->
+        sub_inst i M M' ->
+        sem_block P b M' ess oss ->
+        sem_vars H ys oss ->
+        P_block b M' ess oss ->
+        P_equation bk H M (EqCall ys ck b i es).
+
+    Hypothesis BlockCase:
+      forall b bl P' M H xss yss bk,
+        clock_of xss bk ->
+        find_block b P = Some (bl, P') ->
+        sem_vars H (map fst bl.(b_in)) xss ->
+        sem_vars H (map fst bl.(b_out)) yss ->
+        same_clock xss ->
+        same_clock yss ->
+        (forall n, absent_list (xss n) <-> absent_list (yss n)) ->
+        Forall (sem_equation P bk H M) bl.(b_eqs) ->
+        Forall (P_equation bk H M) bl.(b_eqs) ->
+        P_block b M xss yss.
+
+    Fixpoint sem_equation_mult
+            (b: stream bool) (H: history) (M: memories) (e: equation)
+            (Sem: sem_equation P b H M e) {struct Sem}
+      : P_equation b H M e
+    with sem_block_mult
+           (f: ident) (M: memories) (xss oss: stream (list value))
+           (Sem: sem_block P f M xss oss) {struct Sem}
+         : P_block f M xss oss.
+    Proof.
+      - destruct Sem; eauto.
+      - destruct Sem.
+        eapply BlockCase; eauto.
+        match goal with H: Forall _ _ |- _ => induction H; auto end.
+    Qed.
+
+    Combined Scheme sem_equation_block_ind from
+             sem_equation_mult, sem_block_mult.
+
+  End sem_block_mult.
 
 End SBSEMANTICS.
